

The Binomial Theorem

①

Pascal's Triangle

It is well known that

$$(a+b)^2 = (a^2+b)(a+b) = a^2 + 2ab + b^2$$

Consider the expansions of each of the following!

$$(a+b)^2 = 1a^2 + 2ab + 1b^2$$

$$(a+b)^3 = 1a^3 + 3a^2b + 3ab^2 + 1b^3$$

$$(a+b)^4 = 1a^4 + 4a^3b + 6a^2b^2 + 4ab^3 + 1b^4$$

The Coefficients of a and b can be displayed in an array as:

	1	2	1		
	1	3	3	1	
	1	4	6	4	1

The array of Coefficients displayed above is called Pascal's Triangle, and it is used in determining the Coefficients of the terms of the powers of a binomial expression. Two significant features of a Pascal's Triangle are:

(a) each line of Coefficients is symmetrical

(b) each line of Coefficients can be obtained from the line of Coefficients immediately preceding it.

For completeness, it may be observed that

$$(a+b)^0 = 1 \quad \text{and} \quad (a+b)^1 = 1a + 1b$$

Therefore the table of Coefficients may be written in a triangle as follows:

				1			
			1		1		
		1		2		1	
	1		3		3		1
	1	4		6		4	1
	1	5	10		10	5	1
1	6	15	20	15	6	1	

When an expression is written as a series of terms, it is said to be expanded, and the series is called its expansion. Thus, the expansion of $(a+b)^2$ is $a^2 + 2ab + b^2$. Similarly, we can obtain the coefficients of $(a+b)^4$ from the coefficients of $(a+b)^3$ as follows:

Coefficients of $(a+b)^3$ 1 3 3 1

Coefficients of $(a+b)^4$ 1 4 6 4 1

Hence, the coefficients of $(a+b)^4$ are: 1, 4, 6, 4, 1. Thus,
 $(a+b)^4 = a^4 + 4a^3b + 6a^2b^2 + 4ab^3 + b^4$
 In the expansion of $(a+b)^4$ for example, the following features of the expansion can be enumerated:

- There are 5 terms.
- In each of the terms involved in the expansion, the power of a and b put together is 4. We say that the expansion is homogeneous in a and b .
- While the power of a is in decreasing order, the power of b is in increasing order.

These features are characteristic of the general expansion of $(a+b)^n$.

Ex 1 Using Pascal's triangle, expand and simplify completely: $(2x+3y)^4$

Soln

$$(2x+3y)^4 = (2x)^4 + 4(2x)^3(3y) + 6(2x)^2(3y)^2 + 4(2x)(3y)^3 + (3y)^4$$

$$= 16x^4 + 96x^3y + 216x^2y^2 + 216xy^3 + 81y^4.$$

Ex 2 Using Pascal's triangle, expand and simplify completely $(x-2y)^5$

Soln

Using Pascal's triangle, the coefficients of $(a+b)^5$ derived from the coefficient of $(a+b)^4$ are: 1, 5, 10, 10, 5, 1.

$$(x-2y)^5 = x^5 + 5x^4(-2y) + 10x^3(-2y)^2 + 10x^2(-2y)^3 + 5x(-2y)^4 + (-2y)^5$$

$$= x^5 - 10x^4y + 40x^3y^2 - 80x^2y^3 + 80xy^4 - 32y^5.$$

Ex 3:- Obtain the expansion of $(2n - \frac{1}{2})^4$, in descending powers of n . (3)

Soln

Here $a = 2n$ and $b = -\frac{1}{2}$, therefore the five terms of the expansion will involve

$$(2n)^4, (2n)^3(-\frac{1}{2}), (2n)^2(-\frac{1}{2})^2, (2n)(-\frac{1}{2})^3, (-\frac{1}{2})^4$$

and their coefficients will be respectively

$$1, 4, 6, 4, 1$$

$$\begin{aligned}\therefore (2n - \frac{1}{2})^4 &= (2n)^4 + 4(2n)^3(-\frac{1}{2}) + 6(2n)^2(-\frac{1}{2})^2 + 4(2n)(-\frac{1}{2})^3 + (-\frac{1}{2})^4 \\ &= 16n^4 + 4(8n^3)(-\frac{1}{2}) + 6(4n^2)(\frac{1}{4}) + 4(2n)(-\frac{1}{8}) + \frac{1}{16} \\ &= 16n^4 - 16n^3 + 6n^2 - n + \frac{1}{16} \text{ in descending powers of } n.\end{aligned}$$

Ex 4:- Use Pascal's triangle to obtain the value of $(1.002)^5$, correct to 5 decimal places.

Soln

1.002 may be written as $1 + 0.002$, so that the expansion of $(a+b)^5$ may be used, with $a=1$ and $b=0.002$.

The terms of the expansion will involve

$$1, (0.002), (0.002)^2, (0.002)^3, (0.002)^4, (0.002)^5$$

and the coefficients will be 1, 5, 10, 10, 5, 1.

$$\begin{aligned}\therefore (1.002)^5 &= (1 + 0.002)^5 = 1 + 5(0.002) + 10(0.002)^2 + 10(0.002)^3 + \\ &\quad 5(0.002)^4 + (0.002)^5.\end{aligned}$$

$$\begin{aligned}&= 1 + 0.010 + 0.000040 \\ &= 1.010040, \text{ to 6 d.p.}\end{aligned}$$

Ex 5:- Using Pascal's triangle, simplify, correct to 5 decimal places $(1.01)^4$.

Soln

$$\begin{aligned}(1.01)^4 &= (1 + 0.01)^4 = 1 + 4(0.01) + 6(0.01)^2 + 4(0.01)^3 + (0.01)^4 \\ &= 1 + 0.04 + 0.0006 + 0.000004 + 0.00000001 \\ &= 1.04060 \text{ to 5 d.p.}\end{aligned}$$

Exercises

- Expand:
 (a) $(2x + \frac{1}{3})^5$ (b) $(ax + 3y)^4$ (c) $(4z + 1)^3$ (d) $(x - \frac{1}{2})^5$ (e) $(a^2 - b^2)^5$
- Write down the expansion of $(2+x)^5$ in ascending powers of x . Taking the first ~~three~~ three terms of the expansion, put $x = 0.001$, and find the value of $(2.001)^5$ correct to five places of decimals.
- Write the expansion of $(1 + \frac{1}{4}x)^4$. Taking the first three terms of the expansion, put $x = 0.1$, and find the value of $(1.025)^4$, correct to three places of decimals.
- Expand $(2-x)^6$ in ascending powers of x .

The Binomial Expansion Formula.

Consider the expansion of $(x+y)^5$:

$$\begin{aligned} (x+y)^5 &= (x+y)(x+y)(x+y)(x+y)(x+y) \\ &= x^5 + {}^5C_1 x^4 y + {}^5C_2 x^3 y^2 + {}^5C_3 x^2 y^3 + {}^5C_4 x y^4 + y^5 \end{aligned}$$

$$\Rightarrow (x+y)^n = \underbrace{(x+y)(x+y) \dots (x+y)}_{n \text{ factors}}$$

$$(x+y)^n = x^n + {}^nC_1 x^{n-1} y + {}^nC_2 x^{n-2} y^2 + \dots + {}^nC_r x^{n-r} y^r + \dots + y^n$$

$$\text{But } {}^nC_r = \frac{n!}{(n-r)! r!} = \frac{n(n-1)(n-2) \dots (n-r+1)(n-r)!}{(n-r)! r!}$$

$$= \frac{n(n-1)(n-2) \dots (n-r+1)}{r!}$$

$$\begin{aligned} \text{Hence, } (x+y)^n &= x^n + n x^{n-1} y + \frac{n(n-1)}{2!} x^{n-2} y^2 + \frac{n(n-1)(n-2)}{3!} x^{n-3} y^3 + \dots \\ &\quad + \frac{n(n-1)(n-2) \dots (n-r+1)}{r!} x^{n-r} y^r + \dots + y^n. \end{aligned}$$

It can be shown that the binomial expansion formula holds for positive, negative, integral or any rational value of n , provided there is a restriction on the values of x and y in the expansion of $(x+y)^n$. We shall however consider only the binomial expansion formula for a positive integral n .

Ex 1. Write down the binomial expansion of $(1 + \frac{1}{4}x)^6$ simplifying all the terms.

b). Use the expansion in (a) to evaluate $(1.0025)^6$ correct to five significant figures.

Soln

$$(1 + \frac{1}{4}x)^6 = 1 + {}^6C_1(\frac{1}{4}x)^1 + {}^6C_2(\frac{1}{4}x)^2 + {}^6C_3(\frac{1}{4}x)^3 + {}^6C_4(\frac{1}{4}x)^4 + {}^6C_5(\frac{1}{4}x)^5 + {}^6C_6(\frac{1}{4}x)^6$$

$$= 1 + \frac{6}{1} \cdot \frac{1}{4}x + \frac{6 \times 5}{1 \times 2} (\frac{1}{4}x)^2 + \frac{6 \times 5 \times 4}{1 \times 2 \times 3} (\frac{1}{4}x)^3 + \frac{6 \times 5 \times 4 \times 3}{1 \times 2 \times 3 \times 4} (\frac{1}{4}x)^4 + \frac{6 \times 5 \times 4 \times 3 \times 2}{1 \times 2 \times 3 \times 4 \times 5} (\frac{1}{4}x)^5 + (\frac{1}{4}x)^6$$

$$= 1 + \frac{3}{2}x + \frac{15}{16}x^2 + \frac{5}{16}x^3 + \frac{15}{256}x^4 + \frac{3}{512}x^5 + \frac{1}{4096}x^6$$

$$(b) (1.0025)^6 = (1 + 0.0025)^6 = (1 + \frac{25}{10000})^6 = (1 + \frac{1}{400})^6$$

$$\text{Put } \frac{1}{4}x = \frac{1}{400}$$

$$x = \frac{1}{400} \times 4 = \frac{1}{100} = 0.01$$

$$\therefore (1.0025)^6 = 1 + \frac{3}{2}(0.01) + \frac{15}{16}(0.01)^2 + \frac{5}{16}(0.01)^3 + \frac{15}{256}(0.01)^4 + \dots$$

$$= 1 + 0.015 + 0.00009375 + 0.000003125$$

$$= 1.0150940625$$

$$= 1.0151 \text{ (5 s.f.)}$$